Introduce tighter constraints on benumerate by introducing a bcount predicate
Assuming decidable equality on TItem, bags are now required to keep
track of how many times each items appear; the count function is not
required to be efficient though, since it mostly serves to assert
properties about the behaviour of binsert and benumerate.

The two interesting predicates are
  forall item, bcount beq bempty item = 0
and
  bcount beq (binsert container inserted) item =
  bcount beq container item + (if beq item inserted then 1 else 0).
where beq designates decidable equality.

The three existing implementations of bag have been augmented to show
that they conform to this extended interface.

src/QueryStructure/Refinements/Bags/CachingBags.v
@@ -113,6 +113,18 @@ Definition Cache_bfind
                               updater updater_cacheable) 
            (search_term: TSearchTerm) :=
   bfind (cbag container) search_term.
+
+Definition Cache_bcount
+           {TBag TItem TSearchTerm TCachedValue: Type} 
+           {bag_bag: Bag TBag TItem TSearchTerm}
+           (updater: TItem -> TCachedValue -> TCachedValue)
+           (initial_value: TCachedValue)
+           (updater_cacheable: IsCacheable updater initial_value) 
+           (beq : HasDecidableEquality TItem)
+           (container: @Cache _ _ _ _ bag_bag initial_value 
+                              updater updater_cacheable) 
+           (item: TItem) :=
+  bcount beq (cbag container) item.
          
 Lemma updated_cache_fresh_after_insert :
   forall {TBag TItem TSearchTerm TCachedValue: Type} 
@@ -150,9 +162,9 @@ Definition Cache_binsert
   |}.
 
 Ltac transparent_implementation :=
-  unfold BagInsertEnumerate, BagEnumerateEmpty, BagFindStar, BagFindCorrect;
+  unfold BagInsertEnumerate, BagEnumerateEmpty, BagFindStar, BagFindCorrect, BagInsertCount, BagCountEmpty;
   intros; 
-  first [ apply binsert_enumerate | apply benumerate_empty | apply bfind_correct | apply bfind_star ].
+  first [ apply binsert_enumerate | apply benumerate_empty | apply bfind_correct | apply bfind_star | apply binsert_count | apply bcount_empty ].
 
 Lemma Cache_BagInsertEnumerate :
   forall {TBag TItem TSearchTerm TCachedValue: Type} 
@@ -165,6 +177,18 @@ Lemma Cache_BagInsertEnumerate :
      (Cache_binsert    updater initial_value updater_cacheable).
 Proof. transparent_implementation. Qed.
 
+Lemma Cache_BagInsertCount :
+  forall {TBag TItem TSearchTerm TCachedValue: Type} 
+         {bag_bag: Bag TBag TItem TSearchTerm}
+         (updater: TItem -> TCachedValue -> TCachedValue)
+         (initial_value: TCachedValue)
+         (updater_cacheable: IsCacheable updater initial_value),
+   BagInsertCount
+     (Cache_benumerate updater initial_value updater_cacheable)
+     (Cache_binsert    updater initial_value updater_cacheable)
+     (Cache_bcount     updater initial_value updater_cacheable).
+Proof. transparent_implementation. Qed.
+
 Lemma Cache_BagEnumerateEmpty :
   forall {TBag TItem TSearchTerm TCachedValue: Type} 
          {bag_bag: Bag TBag TItem TSearchTerm}
@@ -174,6 +198,18 @@ Lemma Cache_BagEnumerateEmpty :
  BagEnumerateEmpty
    (Cache_benumerate updater initial_value updater_cacheable)
    (Cache_bempty     updater initial_value updater_cacheable).
+Proof. transparent_implementation. Qed.
+
+Lemma Cache_BagCountEmpty :
+  forall {TBag TItem TSearchTerm TCachedValue: Type} 
+         {bag_bag: Bag TBag TItem TSearchTerm}
+         (updater: TItem -> TCachedValue -> TCachedValue)
+         (initial_value: TCachedValue)
+         (updater_cacheable: IsCacheable updater initial_value),
+ BagCountEmpty
+   (Cache_benumerate updater initial_value updater_cacheable)
+   (Cache_bempty     updater initial_value updater_cacheable)
+   (Cache_bcount     updater initial_value updater_cacheable).
 Proof. transparent_implementation. Qed.
 
 Lemma Cache_BagFindStar :
@@ -219,7 +255,9 @@ Instance CacheAsBag
     binsert    := Cache_binsert    updater initial_value updater_cacheable;
 
     binsert_enumerate := Cache_BagInsertEnumerate updater initial_value updater_cacheable;
+    binsert_count     := Cache_BagInsertCount     updater initial_value updater_cacheable;
     benumerate_empty  := Cache_BagEnumerateEmpty  updater initial_value updater_cacheable;
+    bcount_empty      := Cache_BagCountEmpty      updater initial_value updater_cacheable;
     bfind_star        := Cache_BagFindStar        updater initial_value updater_cacheable;
     bfind_correct     := Cache_BagFindCorrect     updater initial_value updater_cacheable
   |}.
